sparks/playground/Coq/adam-chlipala/hw0.v
@@ -1,5 +1,0 @@
-Check (1 + 1 = 2)
-
-Inductive list : Set :=
-  | nil : list
-  | cons : nat -> list -> list.
